Adds FStar.Int.Cast.Full including FStar.Int.Cast and FStar.UInt128 casts to and from UInt64.t (#1120)
* Fix low-level examples

* Revised OTP

* Add FStar.Int.Cast.Full module including FStar.Int.Cast + UInt128 casts

ulib/FStar.UInt128.fst
@@ -708,11 +708,9 @@ let gte_mask (a b: t) : Pure t
   lt_characterization a b;
   { low = mask; high = mask; }
 
-let uint64_to_uint128 (a: U64.t) = { low = a; high = U64.uint_to_t 0; }
+let uint64_to_uint128 (a:U64.t) = { low = a; high = U64.uint_to_t 0; }
 
-let uint128_to_uint64 (a: t) : Pure U64.t
-    (requires (v a < pow2 64))
-    (ensures (fun r -> U64.v r == v a)) = a.low
+let uint128_to_uint64 (a:t) : b:U64.t{U64.v b == v a % pow2 64} = a.low
 
 let u64_l32_mask: x:U64.t{U64.v x == pow2 32 - 1} = U64.uint_to_t 0xffffffff
 
